LLVM_DS_RBT/Insert/Naive_Insert.thy
@@ -1,10 +1,13 @@
 theory Naive_Insert
-  imports "../Setup"
+  imports 
+    "../Setup"
+    "../Separation_Logic_Solver/Methods"
+    "../Bool_Assn_Setup"
 begin
 
 
 fun rbt_naive_insert ::
-  "('key::linorder, 'val) rbt \<Rightarrow> 'key \<Rightarrow> 'val \<Rightarrow> ('key, 'val) rbt"
+  "('k::linorder, 'v) rbt \<Rightarrow> 'k \<Rightarrow> 'v \<Rightarrow> ('k, 'v) rbt"
   where
     "rbt_naive_insert rbt.Empty k v = Branch color.R rbt.Empty k v rbt.Empty"
   | "rbt_naive_insert (rbt.Branch col lhs k' v' rhs) k v = (
@@ -20,13 +23,11 @@ fun rbt_naive_insert ::
 
 context rbt_impl
 begin
-interpretation llvm_prim_ctrl_setup .
-interpretation llvm_prim_arith_setup .
-interpretation llvm_prim_setup .
+interpretation rbt_impl_deps .
 
 
 partial_function (M) naive_insert :: "
-('ki, 'val::llvm_rep) rbti \<Rightarrow> 'ki \<Rightarrow> 'val \<Rightarrow> ('ki, 'val) rbti llM
+('ki, 'vi) rbti \<Rightarrow> 'ki \<Rightarrow> 'vi \<Rightarrow> ('ki, 'vi) rbti llM
 " where " 
 naive_insert tree_p k v = do {
   if tree_p = null
@@ -58,6 +59,7 @@ naive_insert tree_p k v = do {
       }
       else do {
          key_delete k;
+         value_delete v;
          return tree_p
       }
     }
@@ -67,8 +69,8 @@ naive_insert tree_p k v = do {
 
 lemma naive_insert_correct [vcg_rules]:
   "llvm_htriple
-  (\<upharpoonleft>rbt_assn tree treei ** \<upharpoonleft>key_assn k\<^sub>n ki)
-  (naive_insert treei ki v)
+  (\<upharpoonleft>rbt_assn tree treei ** \<upharpoonleft>key_assn k\<^sub>n ki ** \<upharpoonleft>value_assn v vi)
+  (naive_insert treei ki vi)
   (\<lambda>r. \<upharpoonleft>rbt_assn (rbt_naive_insert tree k\<^sub>n v) r)"
 proof(induction tree arbitrary: treei)
   case Empty
@@ -87,11 +89,54 @@ next
 
   show ?case
     apply (subst naive_insert.simps)
-    by vcg
+    apply vcg
+    done
 qed
 
 
 lemmas [llvm_code] = naive_insert.simps
+
+
+lemma naive_insert_correct_mem [vcg_rules]:
+  "k\<^sub>n \<notin> set (RBT_Impl.keys tree) \<Longrightarrow>
+  llvm_htriple
+  (rbt_assn_mem tree ptrs treei ** \<upharpoonleft>key_assn k\<^sub>n ki ** \<upharpoonleft>value_assn v vi)
+  (naive_insert treei ki vi)
+  (\<lambda>r. EXS n. rbt_assn_mem (rbt_naive_insert tree k\<^sub>n v) (ptrs(k\<^sub>n := Some n)) r)"
+proof(induction tree arbitrary: treei)
+  case Empty
+  note naive_insert_correct[vcg_rules del]
+  then show ?case 
+    apply (subst naive_insert.simps)
+    apply vcg
+    done
+next
+  case (Branch c lhs k v rhs)
+
+  note naive_insert_correct[vcg_rules del]
+  note Branch(1-2)[vcg_rules]
+
+  from Branch(3) show ?case
+    apply (subst naive_insert.simps)
+    apply vcg
+    subgoal (*k\<^sub>n < k*)
+      apply (simp add: fun_upd_def)
+      apply vcg_compat
+      apply (isep_solver_keep isep_intro: ptrs_upd_rbt_assn_mem_sepI)
+        apply simp_all
+      done
+    subgoal (*k\<^sub>n \<ge> k*)
+      apply vcg
+      subgoal (*k\<^sub>n > k*)
+        apply (simp add: fun_upd_def)
+        apply vcg_compat
+        apply (isep_solver_keep isep_intro: ptrs_upd_rbt_assn_mem_sepI)
+          apply simp_all
+        done
+      subgoal (*k\<^sub>n = k -- contradiction*) by vcg
+      done
+    done
+qed
 
 
 end
