LLVM_DS_RBT/Lookup/Lookup.thy
@@ -1,18 +1,18 @@
 theory Lookup
   imports 
     "../Setup"
+    "../Bool_Assn_Setup"
     OptionI
 begin
 
 
 context rbt_impl
 begin
-interpretation llvm_prim_ctrl_setup .
-interpretation llvm_prim_arith_setup .
-interpretation llvm_prim_setup .
+interpretation rbt_impl_deps .
+
 
 partial_function (M) contains :: "
-  ('ki, 'v::llvm_rep) rbti \<Rightarrow> 'ki \<Rightarrow> 1 word llM
+  ('ki, 'vi) rbti \<Rightarrow> 'ki \<Rightarrow> 1 word llM
 " where "
   contains rbtp k = do {
     if rbtp = null
@@ -39,13 +39,12 @@ lemma contains_correct:
   "llvm_htriple
   (\<upharpoonleft>rbt_assn t ti ** \<upharpoonleft>key_assn k ki)
   (contains ti ki)
-  (\<lambda>ri. \<up>(ri = fb (rbt_contains t k)) ** \<upharpoonleft>rbt_assn t ti ** \<upharpoonleft>key_assn k ki)"
+  (\<lambda>ri. \<upharpoonleft>bool.assn (rbt_contains t k) ri ** \<upharpoonleft>rbt_assn t ti ** \<upharpoonleft>key_assn k ki)"
 proof(induction t arbitrary: ti)
   case Empty
   then show ?case
     unfolding rbt_contains_def
     apply (subst contains.simps)
-    apply vcg_monadify
     apply vcg
     done
 next
@@ -55,7 +54,6 @@ next
 
   show ?case
     apply (subst contains.simps)
-    apply vcg_monadify
     apply vcg
     done
 qed
@@ -75,13 +73,11 @@ abbreviation "alloc_opt_none \<equiv> do {
 }"
 
 
-
-
-partial_function (M) lookup :: 
-  "('ki, 'v::llvm_rep) rbti \<Rightarrow> 'ki \<Rightarrow> (('v option_i) ptr) llM" where
+partial_function (M) lookup ::
+  "('ki, 'vi) rbti \<Rightarrow> 'ki \<Rightarrow> 'vi option_i llM" where
   "lookup node_p k = do {
     if node_p = null
-    then alloc_opt_none
+    then return (OPTION_I init 0)
     else do {
       node \<leftarrow> ll_load node_p;
       k_old \<leftarrow> return rbt_node.key node;
@@ -92,7 +88,10 @@ partial_function (M) lookup ::
         k_gt \<leftarrow> lt_impl k_old k;
         if k_gt = 1
         then lookup (rbt_node.right node) k
-        else alloc_opt_of (rbt_node.val node)
+        else do {
+          val_copy \<leftarrow> value_copy (rbt_node.val node);
+          return (OPTION_I val_copy 1)
+        }
       }
     }
   }"
@@ -101,26 +100,24 @@ partial_function (M) lookup ::
 lemmas [llvm_code] = lookup.simps
 
 
-interpretation v_option: option_impl 
-  "mk_assn (\<lambda> v vi. \<up>(v = vi))"
-  .
+interpretation v_option: option_impl value_assn .
 
 
-abbreviation "option_assn \<equiv> v_option.option_assn"
+definition "value_option_assn \<equiv> v_option.option_assn"
 
 
-lemma lookup_correct:
+lemma lookup_correct [vcg_rules]:
   "llvm_htriple
   (\<upharpoonleft>rbt_assn t ti ** \<upharpoonleft>key_assn k ki)
   (lookup ti ki)
-  (\<lambda>ri. (EXS opt.
-            \<upharpoonleft>ll_bpto opt ri **
-            \<upharpoonleft>option_assn (rbt_lookup t k) opt **
-            \<upharpoonleft>rbt_assn t ti **
-            \<upharpoonleft>key_assn k ki))"
+  (\<lambda>opt.
+    \<upharpoonleft>value_option_assn (rbt_lookup t k) opt **
+    \<upharpoonleft>rbt_assn t ti **
+    \<upharpoonleft>key_assn k ki)"
 proof(induction t arbitrary: ti)
   case Empty
   then show ?case
+    unfolding value_option_assn_def
     apply (subst lookup.simps)
     apply vcg
     done
@@ -132,9 +129,38 @@ next
 
   show ?case
     apply (subst lookup.simps)
-    apply vcg_monadify
     apply vcg
-    apply (auto split: if_split)
+    unfolding value_option_assn_def
+    apply vcg
+    done
+qed
+
+
+lemma lookup_correct_mem [vcg_rules]:
+  "llvm_htriple
+  (rbt_assn_mem t ptrs ti ** \<upharpoonleft>key_assn k ki)
+  (lookup ti ki)
+  (\<lambda>opt.
+    \<upharpoonleft>value_option_assn (rbt_lookup t k) opt **
+    rbt_assn_mem t ptrs ti **
+    \<upharpoonleft>key_assn k ki)"
+proof(induction t arbitrary: ti)
+  case Empty
+  then show ?case
+    unfolding value_option_assn_def
+    apply (subst lookup.simps)
+    apply vcg
+    done
+next
+  case (Branch x1 t1 x3 x4 t2)
+
+  note [vcg_rules] = Branch.IH
+  note [simp] = rbt_assn_branch_def
+
+  show ?case
+    apply (subst lookup.simps)
+    apply vcg
+    unfolding value_option_assn_def
     apply vcg
     done
 qed
