LLVM_DS_RBT.thy
@@ -4,18 +4,8 @@ theory LLVM_DS_RBT
   "LLVM_DS_RBT/Insert/Insert"
   "LLVM_DS_RBT/Insert/Naive_Insert"
   "LLVM_DS_RBT/Lookup/Lookup"
-  "LLVM_DS_RBT/Export"
-begin                                     
-
-
-context rbt_impl
+  "LLVM_DS_RBT/Bench_Export"
 begin
-interpretation llvm_prim_ctrl_setup .
-interpretation llvm_prim_arith_setup .
-interpretation llvm_prim_setup .
-
-
-ML_val \<open>Basic_VCG.print_solvers @{context}\<close>
 
 
 end
